Improve bvify by using scalar_tac as a conditional rewriter

backends/lean/Aeneas/Bvify/Bvify.lean
@@ -19,14 +19,70 @@ namespace Aeneas.Bvify
 open Lean Lean.Meta Lean.Parser.Tactic Lean.Elab.Tactic
 open Arith Std
 
-attribute [bvify_simps] ge_iff_le gt_iff_lt decide_eq_true_eq
+def guarded (p q : Prop) := p → q
+
+@[bvify_simps] theorem guarded_true : guarded True q ↔ q := by simp [guarded]
+@[bvify_simps] theorem guarded_same (p : Prop) : guarded p p ↔ True := by simp [guarded, *]
+
+theorem BitVec.lt_pow_ofNat_le {n : Nat} (a b : Nat) (h0 : b < 2^n) (h1 : a ≤ b) :
+  BitVec.ofNat n a ≤ BitVec.ofNat n b := by
+  have : 0 < 2^n := by simp
+  have : a % 2^n = a := by apply Nat.mod_eq_of_lt; omega
+  have : b % 2^n = b := by apply Nat.mod_eq_of_lt; omega
+  simp [*]
+
+/- TODO: we have *two* preconditions, while only one is really needed for the implication
+   in which we're interested - this can be expensive to prove -/
+theorem BitVec.lt_pow_le_iff_ofNat_le {n : Nat} (a b : Nat) (h0 : a < 2^n) (h1 : b < 2^n) :
+  a ≤ b ↔ BitVec.ofNat n a ≤ BitVec.ofNat n b := by
+  constructor <;> intro h2
+  . apply BitVec.lt_pow_ofNat_le <;> assumption
+  . simp at h2
+    have : a % 2^n = a := by apply Nat.mod_eq_of_lt; assumption
+    have : b % 2^n = b := by apply Nat.mod_eq_of_lt; assumption
+    omega
+
+@[bvify_forward a ≤ b]
+theorem BitVec.lt_pow_le_guarded_ofNat_le {n : Nat} (a b : Nat) :
+  guarded (b < 2^n ∧ a ≤ b) (BitVec.ofNat n a ≤ BitVec.ofNat n b) := by
+  sorry
+
+theorem BitVec.lt_pow_ofNat_lt {n : Nat} (a b : Nat) (h0 : b < 2^n) (h0 : a < b) :
+  BitVec.ofNat n a < BitVec.ofNat n b := by
+  have : 0 < 2^n := by simp
+  have : a % 2^n = a := by apply Nat.mod_eq_of_lt; omega
+  have : b % 2^n = b := by apply Nat.mod_eq_of_lt; omega
+  simp [*]
+
+/- TODO: we have *two* preconditions, while only one is really needed for the implication
+   in which we're interested - this can be expensive to prove -/
+theorem BitVec.lt_pow_lt_iff_ofNat_lt {n : Nat} (a b : Nat) (h0 : a < 2^n) (h1 : b < 2^n) :
+  a < b ↔ BitVec.ofNat n a < BitVec.ofNat n b := by
+  constructor <;> intro h2
+  . apply BitVec.lt_pow_ofNat_lt <;> assumption
+  . simp at h2
+    have : a % 2^n = a := by apply Nat.mod_eq_of_lt; assumption
+    have : b % 2^n = b := by apply Nat.mod_eq_of_lt; assumption
+    omega
+
+@[bvify_forward a < b]
+theorem BitVec.lt_pow_lt_guarded_ofNat_lt {n : Nat} (a b : Nat) :
+  guarded (b < 2^n ∧ a < b) (BitVec.ofNat n a < BitVec.ofNat n b) := by
+  sorry
+
+@[bvify_csimps]
+theorem guarded_imp (p q : Prop) (h : p) : guarded p q ↔ q := by simp [guarded, *]
+
+attribute [bvify_simps] ge_iff_le gt_iff_lt decide_eq_true_eq BitVec.ofNat_add
+
+syntax (name := bvify_saturate) "bvify_saturate" term : tactic
 
 /-!
 Some theorems which automatically lift comparisons between machine scalars, without needing the bitwise to be provided by the user.
 -/
 
 attribute [bvify_simps] UScalar.eq_equiv_bv_eq IScalar.eq_equiv_bv_eq
-                        gt_iff_lt ge_iff_le
+                        gt_iff_lt ge_iff_le true_and and_true
 
 @[bvify_simps]
 theorem UScalar.lt_equiv_bv_lt {ty : UScalarTy} (x y : UScalar ty) : x < y ↔ x.bv < y.bv := by rfl
@@ -40,18 +96,39 @@ macro_rules
 | `(tactic| bvify $n $[[$simpArgs,*]]? $[at $location]?) =>
   let args := simpArgs.map (·.getElems) |>.getD #[]
   `(tactic|
-    simp -decide (maxDischargeDepth := 1) only [
-      Int.reduceToNat, Nat.reducePow, Nat.reduceLT,
-      Nat.lt_iff_BitVec_ofNat_lt $n, Nat.le_iff_BitVec_ofNat_le $n,
-      bvify_simps, push_cast, $args,*] $[at $location]?)
+    (simp -decide (maxDischargeDepth := 1) only [
+       Int.reduceToNat, Nat.reducePow, Nat.reduceLT,
+       Nat.lt_iff_BitVec_ofNat_lt $n, Nat.le_iff_BitVec_ofNat_le $n,
+       bvify_simps, push_cast, $args,*] $[at $location]?))
 
 def bvifyTacSimp (loc : Utils.Location) (additionalAsms : List FVarId := []): TacticM Unit := do
+  withMainContext do
   let simpTheorems ← bvifySimpExt.getTheorems
   let simprocs := [``Nat.reducePow, ``Nat.reduceLT]
   Utils.simpAt true {maxDischargeDepth := 1, failIfUnchanged := false} simprocs [simpTheorems] [] [] additionalAsms loc
 
 def bvifyTac (n : Expr) (loc : Utils.Location) : TacticM Unit := do
   Elab.Tactic.focus do
+  withMainContext do
+  trace[Bvify] "Initial goal: {← getMainGoal}"
+  /- -/
+  let toDuplicate ← do
+    match loc with
+    | .wildcard => pure none
+    | .wildcard_dep => throwError "bvifyTac does not support using location `Utils.Location.wildcard_dep`"
+    | .targets hyps type =>
+      if type then throwError "bvifyTac does not support using location `Utils.Location.target` with `type = true`"
+      pure (some hyps)
+  /- First duplicate the propositions in the context: we will need the original ones (which mention
+     integers rather than bit-vectors) for `scalar_tac` to succeed when doing the conditional rewritings. -/
+  let (oldAsms, newAsms) ← Utils.duplicateAssumptions toDuplicate
+  trace[Bvify] "Goal after duplicating the assumptions: {← getMainGoal}"
+  /- Simplify the old assumptions - we keep the new ones for `scalar_tac` -/
+  let loc ← do
+    match loc with
+    | .wildcard => pure (Utils.Location.targets oldAsms true)
+    | .wildcard_dep => throwError "Unreachable"
+    | .targets hyps type => pure (Utils.Location.targets hyps type)
   let addThm (thName : Name) : TacticM FVarId := do
     let thm ← mkAppM thName #[n]
     let thm ← Utils.addDeclTac (← Utils.mkFreshAnonPropUserName) thm (← inferType thm) (asLet := false)
@@ -59,9 +136,50 @@ def bvifyTac (n : Expr) (loc : Utils.Location) : TacticM Unit := do
   let lt_iff ← addThm ``Nat.lt_iff_BitVec_ofNat_lt
   let le_iff ← addThm ``Nat.le_iff_BitVec_ofNat_le
   let eq_iff ← addThm ``Nat.eq_iff_BitVec_ofNat_eq
-  withMainContext do
   bvifyTacSimp loc [lt_iff, le_iff, eq_iff]
-  allGoals do Utils.clearFvarIds #[lt_iff, le_iff, eq_iff]
+  if (← getUnsolvedGoals) == [] then return
+  Utils.clearFVarIds #[lt_iff, le_iff, eq_iff]
+  trace[Bvify] "Goal after simplifying: {← getMainGoal}"
+  /- Small helper to retrieve the old assumptions: when we simplify some assumptions, a new fvar id is
+     introduced for it. Whenever we apply a simplification to the old assumptions, the only way to retrieve
+     their new ids is to go through the context and filter the ids which we know do not come from the duplicated
+     assumptions -/
+  let refreshFVarIds (ignore : Std.HashSet FVarId) : TacticM (Array FVarId) := do
+    withMainContext do
+    let decls := (← (← getLCtx).getDecls).toArray
+    decls.filterMapM fun d => do if (← inferType d.type).isProp ∧ d.fvarId ∉ ignore then pure (some d.fvarId) else pure none
+  /- Saturate the context, by looking only at the new assumptions - we have simplified the old ones.
+
+     In the preprocessing step, we instantiate the value `n` in the theorem -/
+  let preprocessThm (mvars : Array Expr) (_ : Expr) : MetaM Unit :=
+    assert! (mvars.size > 0)
+    mvars[0]!.mvarId!.assign n
+  let newAsmsSet := Std.HashSet.ofArray newAsms
+  let oldAsms ← refreshFVarIds newAsmsSet
+  let oldAsmsSet := Std.HashSet.ofArray oldAsms
+  trace[Bvify] "About to saturate by using the assumptions: {oldAsms.map Expr.fvar}"
+  let satAsms ← Saturate.evalSaturate true preprocessThm [`Aeneas.BvifyTac] (some oldAsms)
+  trace[Bvify] "Goal after saturation (added {satAsms.size} assumptions): {← getMainGoal}"
+  /- Finally, simplify the propositions introduced by by using `saturate` -/
+  let (ref, d) ← tacticToDischarge (← `(tactic|scalar_tac))
+  let dischargeWrapper := Lean.Elab.Tactic.Simp.DischargeWrapper.custom ref d
+  let _ ← dischargeWrapper.with fun discharge? => do
+    -- Initialize the simp context
+    let simpThms ← bvifyCSimpExt.getTheorems
+    let (ctx, simprocs) ← Utils.mkSimpCtx true {maxDischargeDepth := 2, failIfUnchanged := false} .simp
+      [] [simpThms] [] [] []
+    -- Apply the simplifier
+    let _ ← Utils.customSimpLocation ctx simprocs discharge? (.targets satAsms false)
+  trace[Bvify] "Goal after simplifying the saturated assumptions (with scalar_tac as a discharger): {← getMainGoal}"
+  /- Clear the duplicated assumptions -/
+  Utils.clearFVarIds newAsms
+  trace[Bvify] "Goal after clearing the duplicated assumptions: {← getMainGoal}"
+  /- Simplify again the saturated assumptions, this time by using the `bvify_simps` simpset -/
+  let oldNewAsmsSet := oldAsmsSet.union newAsmsSet
+  let satAsms ← refreshFVarIds oldNewAsmsSet
+  bvifyTacSimp (.targets satAsms false) []
+  if (← getUnsolvedGoals) == [] then return
+  trace[Bvify] "Goal after simplifying the saturated assumptions: {← getMainGoal}"
 
 elab "bvify'" n:term : tactic => do
   bvifyTac (← Elab.Term.elabTerm n (Expr.const ``Nat [])) Utils.Location.wildcard
@@ -111,5 +229,15 @@ example (x : U8) (h : x.val < 32) : x.bv < 32#8 := by
 example (a : U32) (h : a.val = 3329) : a.bv = 3329#32 := by
   bvify' 32
   apply h
+
+/--
+info: theorem Aeneas.Bvify.extracted_1 (a b c : U32) (h1 : ↑a + ↑b ≤ 3329 + ↑c) (h0 : c.bv ≤ 3329#32)
+  (_ : a.bv + b.bv ≤ 3329#32 + c.bv) : a.bv + b.bv ≤ 3329#32 + c.bv := sorry
+-/
+#guard_msgs in
+example (a b c : U32) (h0 : c.val ≤ 3329) (h1 : a.val + b.val ≤ 3329 + c.val) : a.bv + b.bv ≤ 3329#32 + c.bv := by
+  bvify' 32
+  extract_goal
+  assumption
 
 end Aeneas.Bvify
