backends/lean/Aeneas/Bvify/Init.lean
@@ -1,11 +1,40 @@
 import Aeneas.Extensions
+import Aeneas.Saturate
 open Lean Meta
 
 namespace Aeneas.Bvify
+
+/-!
+# Tracing
+-/
+
+-- We can't define and use trace classes in the same file
+initialize registerTraceClass `Bvify
+
+/-!
+# Bvify Simpsets
+-/
 
 /-- The `bvify_simps` simp attribute. -/
 initialize bvifySimpExt : SimpExtension ←
   registerSimpAttr `bvify_simps "\
     The `bvify_simps` attribute registers simp lemmas to be used by `bvify`."
+
+/-- The `bvify_csimps` simp attribute, for conditional rewriting which need `scalar_tac` to discharge the preconditions. -/
+initialize bvifyCSimpExt : SimpExtension ←
+  registerSimpAttr `bvify_csimps "\
+    The `bvify_csimps` attribute registers conditional simp lemmas to be used by `bvify`, and for which we use `scalar_tac`
+    to discharge the preconditions."
+
+/-!
+# Bvify Forward Rules
+-/
+-- The sets of forward rules that `bvify` should use
+open Extensions in
+initialize bvifyRuleSet : ListDeclarationExtension Name ← do
+  mkListDeclarationExtension `bvifyRuleSet
+
+macro "bvify_forward" pat:term : attr =>
+  `(attr|aeneas_saturate allow_loose (set := $(Lean.mkIdent `Aeneas.BvifyTac)) (pattern := $pat))
 
 end Aeneas.Bvify
